Update F* and Karamel
Use the newest F* and Karamel.
The FStar.Real.real type no longer supports equality, so we can't use it in the Fir example.

example/Fir.CheckN.fst
@@ -10,44 +10,43 @@ open Pipit.System.Exp
 
 module T = Pipit.Tactics
 
-module R = FStar.Real
+(* TODO move to ratio or fixed-point representation *)
+let tint = Pipit.Prim.Vanilla.TInt
 
-let treal = Pipit.Prim.Vanilla.TReal
+let bibo_rely = Check.exp_of_stream1 #_ #tint
+  (fun i -> (const (-1)) <=^ i /\ i <=^ const 1)
 
-let bibo_rely = Check.exp_of_stream1 #_ #treal
-  (fun i -> (const (R.of_int (-1))) <=^ i /\ i <=^ r1)
-
-let bibo_guar (mul: R.real) = Check.exp_of_stream2 #_ #treal #treal
+let bibo_guar (mul: int) = Check.exp_of_stream2 #_ #tint #tint
   (fun r i -> r <=^ const mul)
 
-type bibo_contract (mul: R.real) =
-  Check.contract table [treal] treal
+type bibo_contract (mul: int) =
+  Check.contract table [tint] tint
     bibo_rely
     (bibo_guar mul)
 
-let r_abs (r: R.real): R.real =
-  R.(if r >=. zero then r else (zero -. r))
+let r_abs (r: int): int =
+  if r >= 0 then r else -r
 
-let rec sum_abs (coeffs: list R.real) =
+let rec sum_abs (coeffs: list int) =
   match coeffs with
-  | [] -> R.zero
-  | c::cs' -> R.(r_abs c +. sum_abs cs')
+  | [] -> 0
+  | c::cs' -> r_abs c + sum_abs cs'
 
 #push-options "--split_queries always"
 
-let rec fir (coeffs: list R.real):
+let rec fir (coeffs: list int):
   bibo_contract (sum_abs coeffs) =
   match coeffs with
   | [] ->
-    let ret = Check.exp_of_stream1 (fun _ -> const 0.0R) in
+    let ret = Check.exp_of_stream1 (fun _ -> const 0) in
 
-    assert (Check.contract_system_induct_k1' bibo_rely (bibo_guar 0.0R) ret) by (T.norm_full ["Fir"]);
+    assert (Check.contract_system_induct_k1' bibo_rely (bibo_guar 0) ret) by (T.norm_full ["Fir"]);
     Check.contract_of_exp1 _ _ ret
   | c :: coeffs' ->
     let fir': bibo_contract (sum_abs coeffs') = fir coeffs' in
     let ret = Check.exp_of_stream1 (fun input ->
-      (input *^ const c) +^ Check.stream_of_contract1 fir' (fby 0.0R input)) in
+      (input *^ const c) +^ Check.stream_of_contract1 fir' (fby 0 input)) in
 
-    assert R.(sum_abs coeffs == r_abs c +. sum_abs coeffs');
+    assert (sum_abs coeffs == r_abs c + sum_abs coeffs');
     assert (Check.contract_system_induct_k1' bibo_rely (bibo_guar (sum_abs coeffs)) ret) by (T.norm_full ["Fir"]);
     Check.contract_of_exp1 _ _ ret
